llm message history

src/main/python/send_to_llm.py
@@ -1,6 +1,7 @@
 import os
 import sys
 from openai import OpenAI
+import json
 
 preamble = "I am trying to complete a proof in Isabelle. Here is my theory file so far:"
 lemma_proof = "I am trying to prove the following lemma:"
@@ -15,42 +16,60 @@ error_request = "Please amend the proof to deal with this error." \
                 "Return only the raw code without any additional text, explanations, or formatting. " \
                 "Do not include ``` or language tags. Just the pure code."
 
-api_key = os.getenv("OPENAI_API_KEY")
+key = os.getenv("OPENAI_API_KEY")
 
 # Initialize client
 client = OpenAI(
     base_url="https://openrouter.ai/api/v1",
-    api_key= api_key
+    api_key= key
 )
 
-def query_llm(prompt: str) -> str:
+def query_llm(prompt: str, history: list) -> tuple[str, list]:
+    
+    history.append({"role": "user", "content": prompt})
+    
     response = client.chat.completions.create(
         model="deepseek/deepseek-r1:free",
-        messages=[{"role": "user", "content": prompt}]
+        messages= history
     )
-    return response.choices[0].message.content.strip()
+
+    reply = response.choices[0].message.content.strip()
+    history.append({"role": "assistant", "content": reply})
+
+    return reply, history
     
 
 if __name__ == "__main__":
+
     # Get arguments from command line
     thy = sys.argv[1]
     lemma = sys.argv[2]
     error = sys.argv[3]
     line = sys.argv[4]
-    mode = int(sys.argv[5])
+    history_json = sys.argv[5]
 
-    if mode == 0:
-        
+    # Open history from json file
+    with open(history_json, "r") as f:
+        chat_history = json.load(f)
+
+    # No chat history means this is the first llm call for this lemma   
+    if len(chat_history) == 0:
+
+        chat_history.append({"role": "system", "content": "You are a theorem proving expert in Isabelle. Prove only the theorems that are given to you. You may use any other proven statement within the .thy file or its imports."})
         input = preamble + "\n" + thy + "\n" + lemma_proof + "\n" + lemma + "\n" + request 
     
-    #Returning failed proof
+    # Returning failed proof
     else:
         
         input = fail_return + "\n" + lemma + "\n" + line_error + "\n" + line + "\n" + error_message + "\n" + error + "\n" + error_request
 
     print("===INPUT===")
-    print(input)   
-    output = query_llm(input)
+    print(input)
+
+    output, chat_history = query_llm(input, chat_history)
+    with open(history_json, "w") as f:
+        json.dump(chat_history, f, indent=2)
+
     print("===OUTPUT===")
     print(output)
 
