src/main/scala/TheoryManager.scala
@@ -1,3 +1,7 @@
+// This file is heavily inspired by the work done on Portal to ISAbelle (PISA)
+// for more information on PISA, go to https://github.com/albertqjiang/Portal-to-ISAbelle
+// FOr this file in particular, go to 
+// https://github.com/albertqjiang/Portal-to-ISAbelle/blob/main/src/main/scala/pisa/utils/TheoryManager.scala
 
 import java.nio.file.{Path, Paths}
 import de.unruh.isabelle.control.{Isabelle, OperationCollection}
