src/main/scala/history.scala
@@ -1,0 +1,18 @@
+import java.io.{File, PrintWriter}
+
+// Functionality for handling the conversation history with the LLM
+
+object history {
+
+    def jsonCreate(lemmaName: String) = {
+    
+        val file = new File(s"history/$lemmaName.json")
+        val writer = new PrintWriter(file)
+        writer.write("[]") // Start with empty JSON array
+        writer.close()
+    }
+
+
+               
+    
+}
