src/main/scala/sledgehammer.scala
@@ -1,3 +1,8 @@
+// This file is heavily inspired by the work done on Portal to ISAbelle (PISA)
+// for more information on PISA, go to https://github.com/albertqjiang/Portal-to-ISAbelle
+// For this file in particular, go to
+// https://github.com/albertqjiang/Portal-to-ISAbelle/blob/main/src/main/scala/pisa/agent/RepHammer.scala
+
 import TheoryManager._
 
 import de.unruh.isabelle.control.Isabelle
@@ -10,6 +15,10 @@ import de.unruh.isabelle.control.{Isabelle, OperationCollection}
 import de.unruh.isabelle.mlvalue.MLValue.compileFunction
 import de.unruh.isabelle.pure.{Position, Theory, TheoryHeader}
 
+import scala.concurrent.Future
+import scala.concurrent.Await
+import scala.concurrent.duration.Duration
+
 import java.nio.file.{Path, Paths}
 
 import de.unruh.isabelle.mlvalue.Implicits._
@@ -18,86 +27,83 @@ import scala.concurrent.ExecutionContext.Implicits.global
 
 object sledgehammer {
 
-    val isabelleHome: Path = Paths.get("/home/eaj123/Isabellm/Isabelle2022")
-    val setup: Setup = Setup(isabelleHome = isabelleHome)
-    val theoryManager: TheoryManager = new TheoryManager(
-        path_to_isa_bin="/home/eaj123/Isabellm/Isabelle2022",
-        wd="/home/eaj123/Isabellm/Test"
-    )
+    // Expose a public method to run Sledgehammer on a theory text
+    def call_sledgehammer (theoryText: String, filePath: String): (Boolean, (String, List[String])) = {
+        
 
-    def main(args: Array[String]): Unit = {
+        val isabelleHome: Path = Paths.get("/home/eaj123/Isabellm/Isabelle2022")
+        val setup: Setup = Setup(isabelleHome = isabelleHome)
+        val theoryManager: TheoryManager = new TheoryManager(
+            path_to_isa_bin="/home/eaj123/Isabellm/Isabelle2022",
+            wd="/home/eaj123/Isabellm/Test"
+        )
 
         implicit val isabelle: Isabelle = new Isabelle(setup)
 
         val theorySource = TheoryManager.Text(
-            """
-            theory test
-  imports Main
-begin
-
-lemma test1: "Suc n  = n"
-proof-
-  have sublem: "Suc n = n+1"
-
-            """,
-            Paths.get("test.thy").toAbsolutePath
+        theoryText,
+        Paths.get(filePath).toAbsolutePath
         )
-        
+
         val thy0 = theoryManager.beginTheory(theorySource)
         val init_toplevel = compileFunction0[ToplevelState]("Toplevel.init_toplevel")
         var toplevel = init_toplevel().force.retrieveNow
 
-
+        // Parse and execute transitions
         val parse_text = compileFunction[Theory, String, List[(Transition.T, String)]](
         """fn (thy, text) => let
-            |  val transitions = Outer_Syntax.parse_text thy (K thy) Position.start text
-            |  fun addtext symbols [tr] =
-            |        [(tr, implode symbols)]
-            |    | addtext _ [] = []
-            |    | addtext symbols (tr::nextTr::trs) = let
-            |        val (this,rest) = Library.chop (Position.distance_of (Toplevel.pos_of tr, Toplevel.pos_of nextTr) |> Option.valOf) symbols
-            |        in (tr, implode this) :: addtext rest (nextTr::trs) end
-            |  in addtext (Symbol.explode text) transitions end""".stripMargin)
+                |  val transitions = Outer_Syntax.parse_text thy (K thy) Position.start text
+                |  fun addtext symbols [tr] =
+                |        [(tr, implode symbols)]
+                |    | addtext _ [] = []
+                |    | addtext symbols (tr::nextTr::trs) = let
+                |        val (this,rest) = Library.chop (Position.distance_of (Toplevel.pos_of tr, Toplevel.pos_of nextTr) |> Option.valOf) symbols
+                |        in (tr, implode this) :: addtext rest (nextTr::trs) end
+                |  in addtext (Symbol.explode text) transitions end""".stripMargin
+        )
 
         val command_exception = compileFunction[Boolean, Transition.T, ToplevelState, ToplevelState](
             "fn (int, tr, st) => Toplevel.command_exception int tr st"
         )
 
         for ((transition, text) <- parse_text(thy0, theorySource.text).force.retrieveNow) {
-            println(s"""Transition: "${text.strip}"""")
             toplevel = command_exception(true, transition, toplevel).retrieveNow.force
         }
 
         val thy_for_sledgehammer = thy0
-    val Sledgehammer: String = thy_for_sledgehammer.importMLStructureNow("Sledgehammer")
-    val Sledgehammer_Commands: String = thy_for_sledgehammer.importMLStructureNow("Sledgehammer_Commands")
-    val Sledgehammer_Prover: String = thy_for_sledgehammer.importMLStructureNow("Sledgehammer_Prover")
+        val Sledgehammer: String = thy_for_sledgehammer.importMLStructureNow("Sledgehammer")
+        val Sledgehammer_Commands: String = thy_for_sledgehammer.importMLStructureNow("Sledgehammer_Commands")
+        val Sledgehammer_Prover: String = thy_for_sledgehammer.importMLStructureNow("Sledgehammer_Prover")
 
-    val normal_with_Sledgehammer: MLFunction4[ToplevelState, Theory, List[String], List[String], (Boolean, (String, List[String]))] =
-      compileFunction[ToplevelState, Theory, List[String], List[String], (Boolean, (String, List[String]))](
-        s""" fn (state, thy, adds, dels) =>
-           |    let
-           |       val override = {add=[],del=[],only=false};
-           |       fun go_run (state, thy) =
-           |          let
-           |             val p_state = Toplevel.proof_of state;
-           |             val ctxt = Proof.context_of p_state;
-           |             val params = ${Sledgehammer_Commands}.default_params thy
-           |                [("provers", "e"),("timeout","30"),("verbose","true")];
-           |             val results = ${Sledgehammer}.run_sledgehammer params ${Sledgehammer_Prover}.Normal NONE 1 override p_state;
-           |             val (result, (outcome, step)) = results;
-           |           in
-           |             (result, (${Sledgehammer}.short_string_of_sledgehammer_outcome outcome, [YXML.content_of step]))
-           |           end;
-           |    in
-           |      Timeout.apply (Time.fromSeconds 35) go_run (state, thy) end
-           |""".stripMargin
-      )
+        val sledgehammerML: MLFunction4[ToplevelState, Theory, List[String], List[String], (Boolean, (String, List[String]))] =
+            compileFunction[ToplevelState, Theory, List[String], List[String], (Boolean, (String, List[String]))](
+                s""" fn (state, thy, adds, dels) =>
+                |    let
+                |       val override = {add=[],del=[],only=false};
+                |       fun go_run (state, thy) =
+                |          let
+                |             val p_state = Toplevel.proof_of state;
+                |             val ctxt = Proof.context_of p_state;
+                |             val params = ${Sledgehammer_Commands}.default_params thy
+                |                [("provers", "e"),("timeout","30"),("verbose","true")];
+                |             val results = ${Sledgehammer}.run_sledgehammer params ${Sledgehammer_Prover}.Normal NONE 1 override p_state;
+                |             val (result, (outcome, step)) = results;
+                |           in
+                |             (result, (${Sledgehammer}.short_string_of_sledgehammer_outcome outcome, [YXML.content_of step]))
+                |           end;
+                |    in
+                |      Timeout.apply (Time.fromSeconds 35) go_run (state, thy) end
+                |""".stripMargin
+        )
 
-    // Apply transitions to toplevel such that it is at a "hammerable" place
-    // Then
-    val result = normal_with_Sledgehammer(toplevel, thy0, List[String](), List[String]()).force.retrieveNow
-    println(result)
+        // Run Sledgehammer
+        val result = sledgehammerML(
+            toplevel,
+            thy0,
+            List[String](), //Added Names
+            List[String]()  //Deleted Names
+        ).force.retrieveNow
 
+        result
     }
 }
