test.thy
@@ -2,8 +2,21 @@ theory test
   imports Main
 begin
 
-lemma test1: "Suc n  = n"
-proof-
-  have sublem: "Suc n = n+1"
+datatype 'a nTree =
+  nNode 'a "'a nTree list"
 
 
+fun nNodes :: "'a nTree \<Rightarrow> nat" where
+  "nNodes (nNode x []) = 1"
+| "nNodes (nNode x (t # ts)) = Suc (foldr (+) (map nNodes (t # ts)) 0)"
+
+fun nHeight :: "'a nTree \<Rightarrow> nat" where
+  "nHeight (nNode x []) = 1"
+| "nHeight (nNode x (t # ts)) = Suc (foldr max (map nHeight (t # ts)) 0)"
+
+lemma subtree_height:
+  assumes "t \<in> set ts" 
+  shows "foldr max (map nHeight ts) 0 \<ge> nHeight t"
+  sorry
+
+end
