test2.thy
@@ -1,0 +1,4 @@
+theory test2
+    imports Main
+begin
+
